chore: AIG.inv -> AIG.invariant

src/Std/Sat/AIG/Relabel.lean
@@ -62,11 +62,11 @@ def relabel (r : α → β) (aig : AIG α) : AIG β :=
   {
     decls,
     cache,
-    inv := by
+    invariant := by
       intro idx lhs rhs linv rinv hbound hgate
       simp [decls] at hgate
       have := Decl.relabel_gate hgate
-      apply aig.inv
+      apply aig.invariant
       assumption
   }
 
@@ -115,7 +115,7 @@ theorem denote_relabel (aig : AIG α) (r : α → β) (start : Nat) {hidx}
     have heq2 := relabel_gate heq1
     rw [denote_idx_gate heq1]
     rw [denote_idx_gate heq2]
-    have := aig.inv (by rw [← relabel_size_eq_size (r := r)]; omega) heq2
+    have := aig.invariant (by rw [← relabel_size_eq_size (r := r)]; omega) heq2
     rw [denote_relabel aig r lhs assign]
     rw [denote_relabel aig r rhs assign]
 
